\documentclass{article}
\usepackage{format}
\title{Introduction to creation and annihilation operators}
\author{Forest Yang}
\date{May 30, 2017}

\begin{document}
\maketitle
Note: when only one subscript $k$ is used for an operator it specifies location $i$ and a spin $\sigma$.
\section{Some relations}
The operator $c_{i\sigma}^\dagger$ creates a spin $\sigma$ particle at position $i$ and the operator $c_{i\sigma}$ annihilates a spin $\sigma$ particle at position $i$. \\
$(c_k^{\dagger})^2 = (c_k)^2 = 0$ follows from the anticommutator relations 
\begin{gather*}
\{c_k^{\dagger}, c_{k'}^{\dagger}\}_{+} = 0 \qquad \{c_k , c_{k'}\}_+ = 0 \qquad \{c_k^{\dagger}, c_{k'}\}_+ = \delta_{kk'}
\end{gather*}
The operator $\hat{n}_k$ is defined as $c_k^{\dagger} c_k$ and can be thought of as counting the number of particles in state $k$. This gives the following commutator relations \\
\begin{equation*} [\hat{n}_k, c_k^{\dagger}] = c_k^{\dagger} \quad \text{``add one then count vs. count then add one" } \end{equation*}
\begin{equation*} [\hat{n}_k, c_k] = -c_k\quad  \text{``subtract one then count vs. count then subtract one"} \end{equation*}
\section{Representing operators}
For a one particle operator $\hat{O}$, we have \begin{equation*} \hat{O} = \sum_{\ell, \sigma, \ell ', \sigma '}\braket{\ell, \sigma| \hat{O} | \ell ' , \sigma '} c_{\ell, \sigma}^{\dagger} c_{\ell', \sigma'} \end{equation*}
because, (?) for some arbitrary $\ell_1, \sigma_1, \ell_2, \sigma_2$, we have 
\begin{align*}
\braket{\ell_1, \sigma_1 | \sum \braket{\ell, \sigma| \hat{O} | \ell ' , \sigma '} c_{\ell, \sigma}^{\dagger} c_{\ell', \sigma'} | \ell_2, \sigma_2} &= \sum \braket{\ell, \sigma| \hat{O} | \ell ' , \sigma '} \bra{\ell_1, \sigma_1} c_{\ell, \sigma}^{\dagger} c_{\ell', \sigma'} \ket{\ell_2, \sigma_2} \\
&= \sum \braket{\ell, \sigma| \hat{O} | \ell ' , \sigma '} \bra{c_{\ell, \sigma} \ell_1, \sigma_1}  \ket{ c_{\ell', \sigma'} \ell_2, \sigma_2} \\
&= \sum \braket{\ell, \sigma| \hat{O} | \ell ' , \sigma '} \braket{0 | 0} \delta_{\ell_1, \ell} \delta_{\sigma_1, \sigma} \delta_{\ell_2, \ell'} \delta_{\sigma_2, \sigma'} \\
&= \braket{\ell_1, \sigma_1 | \hat{O} | \ell_2, \sigma_2}
\end{align*}
\section{Example of a Two Particle Operator}
\begin{align*}
\braket{\ell_1 \sigma_1 \ell_2 \sigma_2| V(|\vec{r}_1 - \vec{r}_2|) |\ell_3 \sigma_3 \ell_4 \sigma_4} &= \frac{1}{V^2} \braket{\sigma_1 | \sigma_4} \braket{\sigma_2 | \sigma_3} \int d^3\vec{r}_2 \int d^3\vec{r}_1 e^{-i(\vec{k}_1 - \vec{k}_4)\cdot \vec{r}_2} V(|\vec{r}_1 - \vec{r}_2|)e^{-i(\vec{k}_2 - \vec{k}_3)\cdot \vec{r}_1}  \\
&= \frac{1}{V^2} \delta_{\sigma_1 \sigma_4}\delta_{\sigma_2 \sigma_3} |\text{det } \vec{J}|   \int  d^3 \vec{r} \int d^3 \vec{R} \, V(r) e^{-i(\vec{k}_1 - \vec{k}_4) \cdot (\vec{R} + \frac{\vec{r}}{2})}e^{-i(\vec{k}_2 - \vec{k}_3) \cdot (\vec{R} - \frac{\vec{r}}{2})}  \\
&= \frac{1}{V^2} \delta_{\sigma_1 \sigma_4}\delta_{\sigma_2 \sigma_3}  \int  d^3 \vec{r} \int d^3 \vec{R} \, V(r) e^{-i(\vec{k}_1 + \vec{k}_2 - \vec{k}_3 - \vec{k}_4) \cdot \vec{R} }e^{-i \frac{1}{2}(\vec{k}_1 -\vec{k}_2 +\vec{k}_3 - \vec{k}_4) \cdot (\vec{r}}  \\
&\stackrel{?}{=}  \frac{1}{V} \delta_{\sigma_1 \sigma_4}\delta_{\sigma_2 \sigma_3} \int d^3 \vec{r} \, \delta(\vec{k}_1 + \vec{k}_2 - \vec{k}_3 - \vec{k}_4) V(r) e^{-i(\vec{k}_1 - \vec{k}_4)} \\
&= \frac{1}{V}  \delta_{\sigma_1 \sigma_4}\delta_{\sigma_2 \sigma_3} \delta(\vec{k}_1 + \vec{k}_2 - \vec{k}_3 - \vec{k}_4) V_{FT} (\vec{k}_1 - \vec{k}_4)
\end{align*}
If $V(r) = \frac{e^2}{r}$ then $V_{FT}(\vec{k}_1 - \vec{k}_4) = \frac{4\pi e^2}{|\vec{k}_1 - \vec{k}_4|} \frac{1}{V}$. Note that $\vec{r}_1 = \vec{R} + \frac{\vec{r}}{2}$ and $\vec{r}_2 = \vec{R} - \frac{\vec{r}}{2}$. Also, \[\vec{J} = \begin{bmatrix} 1 & 0 & 0 & 1/2 & 0 & 0 \\ 0 & 1 & 0 & 0 & 1/2 & 0 \\ 0 & 0 & 1 & 0 & 0 & 1/2 \\
1 & 0 & 0 & -1/2 & 0 & 0 \\ 0 & 1 & 0 & 0 & -1/2 & 0 \\ 0 & 0 & 1 & 0 & 0 & -1/2 \end{bmatrix} \] which has a determinant of -1.

\section{Deriving angular momentum operators}
It was shown that $\hat{L}_z = -ih\frac{\partial }{\partial \phi}$. To get expressions for the other components of angular momentum first note 
\begin{align*}
\frac{\partial}{\partial \phi} &= -r \sin\theta \sin\phi \frac{\partial}{\partial x} + r \sin\theta \cos\phi \frac{\partial}{\partial y} \\
\frac{\partial}{\partial \theta} &= \frac{\partial x}{\partial \theta}\frac{\partial}{\partial x} + \frac{\partial y}{\partial \theta}\frac{\partial}{\partial y} + \frac{\partial z}{\partial \theta}\frac{\partial}{\partial z} \\
&= r\cos\theta\cos\phi\pd{x} + r\cos\theta\sin\phi\pd{y} - r\sin\theta\pd{z} 
\end{align*}
Therefore, 
\begin{align*}
\begin{aligned}
& \cot\theta \cos\phi \pd{\phi} + \sin\phi \pd{\theta} = r\cos\theta \pd{y} - r\sin\theta\sin\phi \pd{z} = z\pd{y} - y\pd{z} = \frac{\hat{L}_x}{i \hbar} && \implies && \hat{L}_x  = i \hbar(\sin\phi \pd{\theta} + \cot\theta \cos\phi \pd{\phi}) \\
& -\cot\theta \sin\phi \pd{\phi} + \cos\phi \pd{\theta} = r\cos\theta \pd{x} - r\sin\theta\cos\phi \pd{z} = z\pd{x} - x\pd{z} = \frac{\hat{L}_y}{-i \hbar} && \implies && \hat{L}_y  = -i \hbar(\cos\phi \pd{\theta} - \cot\theta \sin\phi \pd{\phi})
\end{aligned}
\end{align*}
\section{Homework 12, Exercise 1}
\begin{enumerate}[a)]
\item 
Constructing the spin operators: 
\begin{equation*} 
\hat{S}_z = \frac{1}{2}\sum_{i} \hat{n}_{i\uparrow} - \hat{n}_{i\downarrow} \qquad \hat{S}_+ = \sum_{i} c_{i\uparrow}^{\dagger} c_{i \downarrow} \qquad \hat{S}_- = \sum_{i} c_{i\downarrow}^{\dagger} c_{i \uparrow}
\end{equation*}
Then we have 
\begin{align*}
[\hat{S}_+, \hat{S}_-] &= \sum_{j,k} c_{j \uparrow}^\dagger c_{j \downarrow} c_{k \downarrow}^\dagger c_{k \uparrow} - c_{k \downarrow}^\dagger c_{k \uparrow} c_{j \uparrow}^\dagger c_{j \downarrow} \\
&= \sum_{j,k} [c_{j \uparrow}^\dagger c_{j \downarrow} , c_{k \downarrow}^\dagger c_{k \uparrow} ] \\
&= \sum_{j,k} c_{j \uparrow}^\dagger [c_{j \downarrow}, c_{k \downarrow}^\dagger c_{k \uparrow}] + [c_{j \uparrow}^\dagger, c_{k\downarrow}^\dagger c_{k \uparrow} ] c_{k \downarrow}
\end{align*}
Evaluating the remaining commutators:
\begin{align*}
\begin{aligned}
& [c_{k \downarrow}^\dagger c_{k \uparrow}, c_{j \downarrow}] &=& c_{k \downarrow}^\dagger \{ c_{k\uparrow}, c_{j\downarrow}\}_+ - \{c_{k\downarrow}^\dagger, c_{j\downarrow}\}_+ c_{k\uparrow} &=& -\delta_{jk}c_{k\uparrow} \\
& [c_{k \downarrow}^\dagger c_{k \uparrow}, c_{j \uparrow}^\dagger] &=& c_{k \downarrow}^\dagger \{ c_{k\uparrow},c_{j \uparrow}^\dagger\}_+ - \{c_{k\downarrow}^\dagger, c_{j \uparrow}^\dagger\}_+ c_{k\uparrow} &=& \delta_{jk}c_{k\downarrow}^\dagger
\end{aligned}
\end{align*}
Therefore the last expression for $[\hat{S}_+, \hat{S}_-]$ simplifies to 
\begin{equation*}
 \sum_{j,k} c_{j \uparrow}^\dagger c_{k\uparrow}\delta_{jk} - \delta_{jk}c_{k\downarrow}^\dagger c_{k \downarrow} = \sum_{i} c_{i \uparrow}^\dagger c_{i \uparrow} - c_{i \downarrow}^\dagger c_{i \downarrow} = 2\hat{S}_z
\end{equation*}

Second identity: first, show that if $k \neq k'$ then $[\hat{n}_k, c_{k'}] = [\hat{n}_k, c_{k'}^\dagger] = 0$:
\begin{align*}
[\hat{n}_k, c_{k'}] &= c_k^\dagger c_k c_{k'} - c_{k'}c_k^\dagger c_k \\
&= c_k^\dagger c_k c_{k'} - c_{k'}c_k^\dagger c_k + \{c_k^\dagger, c_{k'}\}c_k \\
&= c_k^\dagger c_k c_{k'} + c_k^\dagger c_{k'} c_k \\
&= c_k^\dagger \{c_k, c_{k'}\} = 0
\end{align*}
And showing that $[\hat{n}_k, c_{k'}^\dagger] = 0$ is similar. \\
Now, evaluating the commutator in the problem for $\hat{S}_+$:
\begin{align*}
[\hat{S}_z, \hat{S}_+] &= \frac{1}{2} \big[\sum_{i,j} (c_{i \uparrow}^\dagger c_{i\uparrow} - c_{i\downarrow}^\dagger c_{i\downarrow})c_{j\uparrow}^\dagger c_{j\downarrow} - c_{j\uparrow}^\dagger c_{j\downarrow}(c_{i \uparrow}^\dagger c_{i\uparrow} - c_{i\downarrow}^\dagger c_{i\downarrow}) \big] \\
&= \frac{1}{2} \sum_{i,j} [\hat{n}_{i\uparrow}, c_{j\uparrow}^\dagger c_{j\downarrow} ] - [\hat{n}_{i\downarrow}, c_{j\uparrow}^\dagger c_{j\downarrow}] \\
&= \frac{1}{2} \sum_{i}  [\hat{n}_{i\uparrow}, c_{i\uparrow}^\dagger c_{i\downarrow} ] - [\hat{n}_{i\downarrow}, c_{i\uparrow}^\dagger c_{i\downarrow}]  \\
&= \frac{1}{2} \sum_{i} c_{i\uparrow}^\dagger [\hat{n}_{i\uparrow} c_{i\downarrow}] + [\hat{n}_{i\uparrow}, c_{i \uparrow}^\dagger] c_{i\downarrow} - (c_{i\uparrow}^\dagger[\hat{n}_{i\downarrow}, c_{i\downarrow}] + [\hat{n}_{i\downarrow}, c_{i\uparrow}^\dagger]c_{i\downarrow}) \\
&= \frac{1}{2} \sum_{i} 0 + c_{i\uparrow}^\dagger c_{i\downarrow} - (c_{i\uparrow}^\dagger (-c_{i \downarrow})  + 0) \\
&= \sum_{i} c_{i\uparrow}^\dagger c_{i\downarrow} = \hat{S}_+
\end{align*}
The procedure for $\hat{S}_-$ is similar.
\item 
\begin{align*}
[\hat{J}_+, \hat{J}_-] &= \sum_{i,j=1}^2 (-1)^{i+j} [c_{i\uparrow}^\dagger c_{i\downarrow}^\dagger, c_{j\downarrow} c_{j\uparrow}]  \\
&= \sum_{i,j=1}^2 (-1)^{i+j}(c_{i\uparrow}^\dagger[c_{i\downarrow}^\dagger, c_{j\downarrow}c_{j\uparrow}] + [c_{i\uparrow}^\dagger, c_{j\downarrow}c_{j\uparrow}]c_{i\downarrow}^\dagger) \\
&= \sum_{i,j=1}^2 (-1)^{i+j} (c_{i\uparrow}^\dagger c_{j\uparrow} \delta_{ij} - c_{j\downarrow} c_{i\downarrow}^\dagger \delta_{ij}) \\ 
&= \sum_{i=1}^2 (-1)^{2i}(c_{i\uparrow}^\dagger c_{i\uparrow} - c_{i\downarrow}c_{i\downarrow} + \{c_{i\downarrow}^\dagger, c_{i\downarrow}\} - 1) \\
&= \sum_{i=1}^2 c_{i\uparrow}^\dagger c_{i\uparrow} + c_{i\downarrow}^\dagger c_{i\downarrow} - 1 = 2\hat{J}_z
\end{align*}
Second identity:
\begin{align*}
[\hat{J}_z, \hat{J}_+] &= \frac{1}{2} \sum_{i,j=1}^2 (-1)^{j+1} [c_{i\uparrow}^\dagger c_{i\uparrow} + c_{i\downarrow}^\dagger c_{i\downarrow}, c_{j\uparrow}^\dagger c_{j \downarrow}^\dagger] \\
&= \frac{1}{2}\sum_{i,j=1}^2 (-1)^{j+1} ([\hat{n}_{i\uparrow}, c_{j\uparrow}^\dagger c_{j\downarrow}^\dagger] + [\hat{n}_{i\downarrow}, c_{j\uparrow}^\dagger c_{j\downarrow}^\dagger]) \\
&= \frac{1}{2} \sum_{i,j=1}^2 (-1)^{j+1} (c_{j\uparrow}^\dagger [\hat{n}_{i\uparrow}, c_{i\downarrow}^\dagger] + [\hat{n}_{i\uparrow}, c_{j\uparrow}^\dagger] c_{j\downarrow}^\dagger  + c_{j\uparrow}^\dagger [\hat{n}_{i\downarrow}, c_{i\downarrow}^\dagger] + [\hat{n}_{i\downarrow}, c_{j\uparrow}^\dagger]c_{j\downarrow}^\dagger) \\
&= \frac{1}{2} \sum_{i,j=1}^2 (-1)^{j+1} (0 + c_{j\uparrow}^\dagger c_{j\downarrow}^\dagger \delta_{ij} + c_{j\uparrow}^\dagger c_{j\downarrow} + 0) \\
&= \sum_{i=1}^2 (-1)^{i+1} c_{i\uparrow}^\dagger c_{i\downarrow}^\dagger = \hat{J}_+
\end{align*}
Again the calculation for $\hat{J}_- $ is similar. \\
$[\hat{J}_z, \hat{S}_z] = 0$ because once expanded the commutator yields a sum of commutators of the form $[\hat{n}_k, \hat{n}_{k'}]$. If $k=k'$ clearly the commutator is 0, otherwise it is 0 due to the earlier result that $[\hat{n}_k, c_{k'}] = [\hat{n}_k, c_{k'}^\dagger] = 0$ if $k \neq k'$. \\
\begin{align*}
[\hat{J}_z, \hat{S}_+] &= \frac{1}{2} \sum_{i,j} [n_{i\uparrow}, c_{j\uparrow}^\dagger c_{j\downarrow}] + [\hat{n}_{i\downarrow}, c_{j\uparrow}^\dagger c_{j\downarrow} ] \\
&= \frac{1}{2} \sum_{ij} c_{j\uparrow}^\dagger [n_{i\uparrow}, c_{j\downarrow}] + [\hat{n}_{i\uparrow} c_{j\uparrow}^\dagger + c_{j\uparrow}^\dagger [\hat{n}_{i\downarrow}, c_{j\downarrow}] + [\hat{n}_{i \downarrow}, c_{j\uparrow}^\dagger] c_{j\downarrow} \\
&= \frac{1}{2} \sum_{ij} 0 + \delta_{ij} c_{j\uparrow}^\dagger c_{j \downarrow} - \delta_{ij} c_{j\uparrow}^\dagger c_{j \downarrow} + 0 = 0
\end{align*}
\begin{align*}
[\hat{S}_z, \hat{J}_+] &= \frac{1}{2} \sum_{i,j} (-1)^{j+1} ([\hat{n}_{i\uparrow}, c_{j\uparrow}^\dagger c_{j\downarrow}^\dagger] - [\hat{n}_{i\downarrow}, c_{j\uparrow}^\dagger c_{j \downarrow}^\dagger]) \\
&= \frac{1}{2} \sum_{i,j} (-1)^{j+1} ( c_{j\uparrow}^\dagger [\hat{n}_{i\uparrow}, c_{j\downarrow}^\dagger] + [\hat{n}_{i\uparrow}, c_{j\uparrow}^\dagger] c_{j\downarrow}^\dagger - c_{j\uparrow}^\dagger [\hat{n}_{i\downarrow}, c_{j\downarrow}^\dagger] - [\hat{n}_{i\downarrow}, c_{j\uparrow}^\dagger]c_{j\downarrow}^\dagger) \\
&= 0
\end{align*}
\begin{align*}
[\hat{J}_+, \hat{S}_+] &= \sum_{i,j} (-1)^{i+1} [c_{i\uparrow}^\dagger c_{i\downarrow}^\dagger, c_{j\uparrow}^\dagger c_{j\downarrow}] \\
&= \sum_{i,j} (-1)^{i+1}(c_{j\uparrow}^\dagger[c_{i\uparrow}^\dagger c_{i\downarrow}^\dagger, c_{j\downarrow}] + [c_{i\uparrow}^\dagger c_{i \downarrow}^\dagger, c_{j\uparrow}^\dagger] c_{j\downarrow}) \\
&= \sum_{i,j} (-1)^{i+1}\big[c_{j\uparrow}^\dagger (c_{i\uparrow}^\dagger \{ c_{i\downarrow}^\dagger, c_{j\downarrow} \} - \{c_{i\uparrow}^\dagger, c_{j\downarrow} \} c_{i\downarrow}^\dagger) + (c_{i\uparrow}^\dagger \{ c_{i\downarrow}^\dagger, c_{j\uparrow}^\dagger \} - \{ c_{i\uparrow}^\dagger, c_{j\uparrow}^\dagger\} c_{i\downarrow}^\dagger) c_{j\downarrow} \big] \\
&= \sum_{i} (-1)^{i+1} (c_{i\uparrow}^\dagger)^2 = 0
\end{align*}
\begin{align*}
[\hat{J}_+, \hat{S}_-] &= \sum_{i,j} (-1)^{i+1} [c_{i\uparrow}^\dagger c_{i\downarrow}^\dagger, c_{j\downarrow}^\dagger c_{j\uparrow}] \\
&= \sum_{i,j} (-1)^{i+1}(c_{j\downarrow}^\dagger[c_{i\uparrow}^\dagger c_{i\downarrow}^\dagger, c_{j\uparrow}] + [c_{i\uparrow}^\dagger c_{i\downarrow}^\dagger, c_{j\downarrow}^\dagger]c_{j\uparrow}) \\
&= \sum_{i,j} (-1)^{i+1}\big[c_{j\downarrow}^\dagger (c_{i\uparrow}^\dagger \{ c_{i\downarrow}^\dagger, c_{j\uparrow} \} - \{ c_{i\uparrow}^\dagger, c_{j\uparrow} \} c_{j\downarrow}^\dagger) + (c_{i\uparrow}^\dagger \{ c_{i\downarrow}^\dagger, c_{j\downarrow}^\dagger \} - \{c_{i\uparrow}^\dagger, c_{j\downarrow}^\dagger \} c_{i\downarrow}^\dagger) c_{j\uparrow} \big] \\
&= \sum_{i} (-1)^i (c_{i\downarrow}^\dagger)^2 = 0
\end{align*}
\end{enumerate}
\end{document}